Make sure renamed apart annotations are not extracted

theories/DCVE.v
@@ -2,7 +2,7 @@ Require Import Util AllInRel MapDefined IL Sim Status Annotation.
 Require Import Rename RenamedApart RenamedApart_Liveness AppExpFree.
 Require UCE DVE.
 Require Import Reachability ReachabilityAnalysis ReachabilityAnalysisCorrect.
-Require Import TrueLiveness.
+Require Import TrueLiveness VarP.
 Require LivenessAnalysis LivenessAnalysisCorrect.
 
 Arguments sim S {H} S' {H0} r t _ _.
@@ -13,6 +13,7 @@ Notation "'co_ra' x" := (snd x) (at level 10, only parsing).
 
 Hint Resolve reachability_SC_S correct.
 
+(*
 Definition DCVE i (s:IL.stmt) (ra:ann (⦃var⦄ * ⦃var⦄)) : stmt * ann ⦃var⦄ * ann (⦃var⦄ * ⦃var⦄) :=
   let uc := reachabilityAnalysis s in
   let s_uce := UCE.compile nil s uc in
@@ -21,6 +22,22 @@ Definition DCVE i (s:IL.stmt) (ra:ann (⦃var⦄ * ⦃var⦄)) : stmt * ann ⦃v
   let s_dve := DVE.compile nil s_uce tlv in
   let ra_dve := DVE.compile_renamedApart s_uce tlv ra_uce (fst (getAnn ra_uce)) in
   (s_dve, DVE.compile_live s_uce tlv ∅, ra_dve).
+*)
+
+Definition DCVE i (s:IL.stmt) : stmt * ann ⦃var⦄ :=
+  let uc := reachabilityAnalysis s in
+  let s_uce := UCE.compile nil s uc in
+  let tlv := LivenessAnalysis.livenessAnalysis i s_uce in
+  let s_dve := DVE.compile nil s_uce tlv in
+  (s_dve, DVE.compile_live s_uce tlv ∅).
+
+Definition DCVEra i (s:IL.stmt) (ra:ann (⦃var⦄ * ⦃var⦄)) : ann (⦃var⦄ * ⦃var⦄) :=
+  let uc := reachabilityAnalysis s in
+  let s_uce := UCE.compile nil s uc in
+  let ra_uce := UCE.compile_renamedApart s ra uc in
+  let tlv := LivenessAnalysis.livenessAnalysis i s_uce in
+  let ra_dve := DVE.compile_renamedApart s_uce tlv ra_uce (fst (getAnn ra_uce)) in
+  ra_dve.
 
 
 Lemma DCVE_true_live_sound i s (PM:LabelsDefined.paramsMatch s nil)
@@ -43,8 +60,8 @@ Qed.
 
 Hint Resolve DCVE_UCE_params_match.
 
-Lemma DCVE_live i (ili:IL.stmt) (PM:LabelsDefined.paramsMatch ili nil) ra
-  : Liveness.live_sound i nil nil (co_s (DCVE i ili ra)) (co_lv (DCVE i ili ra)).
+Lemma DCVE_live i (ili:IL.stmt) (PM:LabelsDefined.paramsMatch ili nil)
+  : Liveness.live_sound i nil nil (fst (DCVE i ili)) (snd (DCVE i ili)).
 Proof.
   unfold DCVE. simpl.
   eapply (@DVE.dve_live _ nil nil).
@@ -60,9 +77,9 @@ Qed.
 
 Hint Resolve DCVE_UCE_renamedApart.
 
-Lemma DCVE_noUC b i ili (PM:LabelsDefined.paramsMatch ili nil) ra
+Lemma DCVE_noUC b i ili (PM:LabelsDefined.paramsMatch ili nil)
   : LabelsDefined.noUnreachableCode (LabelsDefined.isCalled b)
-                                    (co_s (DCVE i ili ra)).
+                                    (fst (DCVE i ili)).
 Proof.
   intros. subst. simpl.
   eapply LabelsDefined.noUnreachableCode_mono.
@@ -73,8 +90,8 @@ Proof.
   - intros; eapply LabelsDefined.trueIsCalled_isCalled; eauto.
 Qed.
 
-Lemma DCVE_occurVars i s (PM:LabelsDefined.paramsMatch s nil) ra
-  : getAnn (co_lv (DCVE i s ra)) ⊆ occurVars s.
+Lemma DCVE_occurVars i s (PM:LabelsDefined.paramsMatch s nil)
+  : getAnn (snd (DCVE i s)) ⊆ occurVars s.
 Proof.
   simpl.
   rewrite DVE.compile_live_incl_empty; eauto.
@@ -82,9 +99,9 @@ Proof.
   eapply UCE.compile_occurVars.
 Qed.
 
-Lemma DCVE_correct_I (ili:IL.stmt) (E:onv val) ra
+Lemma DCVE_correct_I (ili:IL.stmt) (E:onv val)
   (PM:LabelsDefined.paramsMatch ili nil)
-  : sim I.state I.state bot3 Sim (nil, E, ili) (nil, E, co_s (DCVE Liveness.Imperative ili ra)).
+  : sim I.state I.state bot3 Sim (nil, E, ili) (nil, E, fst (DCVE Liveness.Imperative ili)).
 Proof.
   intros. subst. unfold DCVE.
   simpl in *.
@@ -110,10 +127,10 @@ Proof.
   eapply DVE.I.sim_DVE; [ reflexivity | eapply LivenessAnalysisCorrect.correct; eauto ].
 Qed.
 
-Lemma DCVE_correct_F (ilf:IL.stmt) (E:onv val) ra
+Lemma DCVE_correct_F (ilf:IL.stmt) (E:onv val)
   (PM:LabelsDefined.paramsMatch ilf nil)
   : defined_on (IL.occurVars ilf) E
-    -> sim F.state F.state bot3 Sim (nil, E, ilf) (nil, E, co_s (DCVE Liveness.Functional ilf ra)).
+    -> sim F.state F.state bot3 Sim (nil, E, ilf) (nil, E, fst (DCVE Liveness.Functional ilf)).
 Proof.
   intros. subst. unfold DCVE.
   simpl in *.
@@ -148,7 +165,7 @@ Definition compile_renamedApart i s ra :=
 
 Lemma DCVE_renamedApart i s ra (PM:LabelsDefined.paramsMatch s nil)
   : renamedApart s ra
-    -> renamedApart (co_s (DCVE i s ra)) (co_ra (DCVE i s ra)).
+    -> renamedApart (fst (DCVE i s)) (DCVEra i s ra).
 Proof.
   intros. simpl.
   exploit (@LivenessAnalysisCorrect.correct i); eauto.
@@ -186,7 +203,7 @@ Qed.
 
 Lemma DCVE_live_incl i s ra (RA:renamedApart s ra) (PM:LabelsDefined.paramsMatch s nil)
   : ann_R (fun (x : ⦃nat⦄) (y : ⦃nat⦄ * ⦃nat⦄) => x ⊆ fst y)
-          (co_lv (DCVE i s ra)) (co_ra (DCVE i s ra)).
+          (snd (DCVE i s)) (DCVEra i s ra).
 Proof.
   unfold DCVE; simpl.
   eapply DVE.DVE_live_incl.
@@ -201,16 +218,16 @@ Proof.
   - eauto with cset.
 Qed.
 
-Lemma DCVE_paramsMatch i s ra (RA:renamedApart s ra) (PM:LabelsDefined.paramsMatch s nil)
-  : LabelsDefined.paramsMatch (co_s (DCVE i s ra)) nil.
+Lemma DCVE_paramsMatch i s (PM:LabelsDefined.paramsMatch s nil)
+  : LabelsDefined.paramsMatch (fst (DCVE i s)) nil.
 Proof.
   unfold DCVE; simpl.
   exploit (@DVE.DVE_paramsMatch i nil nil); eauto.
 Qed.
 
-Lemma DCVE_app_expfree i s ra
+Lemma DCVE_app_expfree i s
       (AEF:app_expfree s)
-  : app_expfree (co_s (DCVE i s ra)).
+  : app_expfree (fst (DCVE i s)).
 Proof.
   simpl.
   eapply DVE.DVE_app_expfree.
@@ -219,10 +236,10 @@ Qed.
 
 Lemma DCVE_ra_fst s ra
       (PM:LabelsDefined.paramsMatch s nil) (RA:renamedApart s ra)
-  : fst (getAnn (snd (DCVE Liveness.Imperative s ra)))
+  : fst (getAnn (DCVEra Liveness.Imperative s ra))
         [=] fst (getAnn ra).
 Proof.
-  simpl.
+  unfold DCVEra.
   rewrite DVE.fst_getAnn_renamedApart'; eauto.
   exploit UCE.compile_renamedApart_pes; eauto.
   + rewrite H. reflexivity.
@@ -230,20 +247,18 @@ Qed.
 
 Lemma DCVE_ra_snd s ra
       (PM:LabelsDefined.paramsMatch s nil) (RA:renamedApart s ra)
-  : snd (getAnn (snd (DCVE Liveness.Imperative s ra)))
+  : snd (getAnn (DCVEra Liveness.Imperative s ra))
         ⊆ snd (getAnn ra).
 Proof.
-  simpl.
+  unfold DCVEra.
   rewrite DVE.snd_getAnn_renamedApart; eauto.
   exploit UCE.compile_renamedApart_pes; eauto.
   + rewrite H. reflexivity.
 Qed.
 
-Require Import VarP.
-
-Lemma DCVE_var_P i (P:nat -> Prop) (s:stmt) ra (PM:LabelsDefined.paramsMatch s nil)
+Lemma DCVE_var_P i (P:nat -> Prop) (s:stmt) (PM:LabelsDefined.paramsMatch s nil)
   (VP:var_P P s)
-  : var_P P (co_s (DCVE i s ra)).
+  : var_P P (fst (DCVE i s)).
 Proof.
   simpl.
   eapply (@DVE.DVE_var_P i _ nil nil); eauto.
